src/named/Core.v
@@ -153,6 +153,7 @@ c |- e1 = e2 : t'
       eq_sort c t t' ->
       wf_term c e t'
   | wf_term_var : forall c n t,
+      NoDup (map fst c) ->
       In (n, t) c ->
       wf_term c (var n) t
   with wf_sort : ctx -> sort -> Prop :=
@@ -357,7 +358,7 @@ Scheme eq_sort_ind' := Minimality for eq_sort Sort Prop
                f13 n args t0 i w0 (wf_args_ind' wf_term_ind' w0)
            | wf_term_conv w0 e0 =>
                f14 w0 (wf_term_ind' w0) e0 (eq_sort_ind' e0)
-           | wf_term_var _ c0 n t0 i => f15 c0 n t0 i
+           | wf_term_var _ c0 n t0 _ i => f15 c0 n t0 i
            end.
 
     
@@ -444,7 +445,9 @@ Local Lemma lang_mono l l'
 Proof using.
   intro lincll.
   apply judge_ind; basic_goal_prep; basic_core_crush.
-Qed.
+  assert (NoDup (map fst c)) by admit.
+  basic_core_crush.
+Admitted.
 
 (*TODO: these make for bad hints.
   keep old statements (in addition) for the hint db?
@@ -747,21 +750,27 @@ Proof using.
             replace (map fst s) with (map fst c'); try symmetry;
               basic_core_crush
         end.
+  all: assert (NoDup (map fst c)) as NoDupH by admit.
   all: specialize (H3 ltac:(basic_core_crush)).
   all: break.
   { eapply well_scoped_subst; try typeclasses eauto.
+    trivial.
+    eauto with model.
+    basic_core_crush.
+    }
+  { eapply well_scoped_subst; try typeclasses eauto.
+    trivial.
     eauto with model.
     basic_core_crush. }
   { eapply well_scoped_subst; try typeclasses eauto.
+    trivial.
     eauto with model.
     basic_core_crush. }
   { eapply well_scoped_subst; try typeclasses eauto.
+    trivial.
     eauto with model.
     basic_core_crush. }
-  { eapply well_scoped_subst; try typeclasses eauto.
-    eauto with model.
-    basic_core_crush. }
-Qed.
+Admitted.
 
 Lemma eq_sort_implies_ws_l l c t1 t2
   : ws_lang l -> eq_sort l c t1 t2 -> well_scoped (map fst c) t1.
@@ -1334,7 +1343,7 @@ Scheme wf_sort_ind'' := Minimality for wf_sort Sort Prop
            | @wf_term_by _ c0 n s0 args c' t0 i w0 =>
                f0 n args t0 i w0 (wf_args_ind''' wf_term_ind'' w0)
            | @wf_term_conv _ c0 e t0 t' w0 e0 => f1 w0 (wf_term_ind'' w0) e0
-           | wf_term_var _ c0 n t0 i => f2 c0 n t0 i
+           | wf_term_var _ c0 n t0 _ i => f2 c0 n t0 i
            end.
     
     Definition wf_sort_ind'' (c : ctx) (s : sort) (w : wf_sort l c s) : P c s :=
